ref_impl/NSMain__main_main.fst
@@ -1,78 +1,187 @@
 module NSMain__main_main
 open BosqueOption
 
-let bTypeStringType_BAnyType =             (BTypedStringType BAnyType)
-let bUnionType_BBoolType_BIntType_BNoneType_bTypeStringType_BAnyType =             (BUnionType BBoolType (BUnionType BIntType (BUnionType BNoneType bTypeStringType_BAnyType)))
-let bUnionType_BIntType_BNoneType =             (BUnionType BIntType BNoneType)
-let bUnionType_bTupleType_false3(SCons BIntType (SCons BBoolType (SCons BIntType SNil)))_bTupleType_true4(SCons BIntType (SCons BBoolType (SCons BIntType (SCons BBoolType SNil)))) =             (BUnionType bTupleType_false3(SCons BIntType (SCons BBoolType (SCons BIntType SNil))) bTupleType_true4(SCons BIntType (SCons BBoolType (SCons BIntType (SCons BBoolType SNil)))))
+let bTypeStringType_BAnyType = (BTypedStringType BAnyType)
+let bTypeStringType_BNoneType = (BTypedStringType BNoneType)
 
-val nSMain__identityUnion : (x:bosqueTerm{subtypeOf bUnionType_BBoolType_BIntType_BNoneType_bTypeStringType_BAnyType (getType x)}) -> Tot (x:bosqueTerm{subtypeOf bUnionType_BBoolType_BIntType_BNoneType_bTypeStringType_BAnyType (getType x)})
-let nSMain__identityUnion x = 
+let bUnionType_bUnionType_BNoneType_bTypeStringType_BNoneType = (BUnionType BNoneType bTypeStringType_BNoneType)
+
+
+
+val nSMain__id : (x:bosqueTerm{subtypeOf BIntType (getType x)}) -> Tot (x:bosqueTerm{subtypeOf BIntType (getType x)})
+let nSMain__id x = 
     let __ir_ret__ = x in 
         let _return_ = __ir_ret__ in 
             _return_
 
-val nSMain__max : (x:bosqueTerm{subtypeOf bUnionType_BIntType_BNoneType (getType x)}) -> (x:bosqueTerm{subtypeOf BIntType (getType x)}) -> Tot (x:bosqueTerm{subtypeOf BIntType (getType x)})
-let nSMain__max x y = 
-    let __tmp_0 = true in 
-        if (op_Equality __tmp_0 true) then 
-            let __ir_ret___2 = y in 
-                let __ir_ret___3 = __ir_ret___2 in 
-                    let _return_ = __ir_ret___3 in 
-                        _return_
-        else 
-            let __tmp_4 = (op_GreaterThanOrEqual x y) in 
-                if (op_Equality __tmp_4 true) then 
-                    let __ir_ret___1 = x in 
-                        let __ir_ret___3 = __ir_ret___1 in 
+val nSMain__id : (x:bosqueTerm{subtypeOf BIntType (getType x)}) -> Tot (x:bosqueTerm{subtypeOf BIntType (getType x)})
+let nSMain__id x = 
+    let __ir_ret__ = x in 
+        let _return_ = __ir_ret__ in 
+            _return_
+
+val nSMain__Board__markCellWith : (x:bosqueTerm{subtypeOf BNoneType (getType x)}) -> (x:bosqueTerm{subtypeOf BIntType (getType x)}) -> (x:bosqueTerm{subtypeOf BIntType (getType x)}) -> (x:bosqueTerm{subtypeOf bTypeStringType_BNoneType (getType x)}) -> Tot (x:bosqueTerm{subtypeOf BNoneType (getType x)})
+let nSMain__Board__markCellWith this x y mark = 
+    let _MIRAccessFromField = 0 in 
+        let __tmp_9 = (op_Multiply y 3) in 
+            let __tmp_7 = (op_Addition x __tmp_9) in 
+                let __tmp_6 = (nSCore__List__set<T=NSCore__None|NSCore__String<NSMain__PlayerMark>> __tmp_5 __tmp_7 mark) in 
+                    let _MIRModifyWithFields = 0 in 
+                        let __ir_ret__ = __tmp_2 in 
+                            let _return_ = __ir_ret__ in 
+                                _return_
+
+val nSMain__id : (x:bosqueTerm{subtypeOf BIntType (getType x)}) -> Tot (x:bosqueTerm{subtypeOf BIntType (getType x)})
+let nSMain__id x = 
+    let __ir_ret__ = x in 
+        let _return_ = __ir_ret__ in 
+            _return_
+
+val nSMain__Board__checkSingleWinner : (x:bosqueTerm{subtypeOf BNoneType (getType x)}) -> (x:bosqueTerm{subtypeOf bTypeStringType_BNoneType (getType x)}) -> Tot (x:bosqueTerm{subtypeOf BBoolType (getType x)})
+let nSMain__Board__checkSingleWinner this mark = 
+    let _MIRAccessConstantValue = 0 in 
+        let __tmp_2 = (nSCore__List__any<T=NSCore__List<[NSCore__Int, NSCore__Int]>>[/Users/joseabelcastellanosjoo/BosqueLanguage/ref_impl/src/test/apps/tictactoe/main.bsq%78%0] __tmp_1 mark this) in 
+            let __ir_ret__ = __tmp_2 in 
+                let _return_ = __ir_ret__ in 
+                    _return_
+
+val nSMain__Board__checkForWinner : (x:bosqueTerm{subtypeOf BNoneType (getType x)}) -> Tot (x:bosqueTerm{subtypeOf bUnionType_BNoneType_bTypeStringType_BNoneType (getType x)})
+let nSMain__Board__checkForWinner this = 
+    let _MIRAccessConstantValue = 0 in 
+        let __tmp_0 = (nSMain__Board__checkSingleWinner this __tmp_2) in 
+            if (op_Equality __tmp_0 true) then 
+                let _MIRAccessConstantValue = 0 in 
+                    let __ir_ret___2 = __tmp_3 in 
+                        let __ir_ret___3 = __ir_ret___2 in 
                             let _return_ = __ir_ret___3 in 
                                 _return_
+            else 
+                let _MIRAccessConstantValue = 0 in 
+                    let __tmp_4 = (nSMain__Board__checkSingleWinner this __tmp_6) in 
+                        if (op_Equality __tmp_4 true) then 
+                            let _MIRAccessConstantValue = 0 in 
+                                let __ir_ret___1 = __tmp_7 in 
+                                    let __ir_ret___3 = __ir_ret___1 in 
+                                        let _return_ = __ir_ret___3 in 
+                                            _return_
+                        else 
+                            let __ir_ret__ = none in 
+                                let __ir_ret___3 = __ir_ret__ in 
+                                    let _return_ = __ir_ret___3 in 
+                                        _return_
+
+val nSMain__id : (x:bosqueTerm{subtypeOf BIntType (getType x)}) -> Tot (x:bosqueTerm{subtypeOf BIntType (getType x)})
+let nSMain__id x = 
+    let __ir_ret__ = x in 
+        let _return_ = __ir_ret__ in 
+            _return_
+
+val nSMain__Board__getOpenCells : (x:bosqueTerm{subtypeOf BNoneType (getType x)}) -> Tot (x:bosqueTerm{subtypeOf BNoneType (getType x)})
+let nSMain__Board__getOpenCells this = 
+    let _MIRAccessConstantValue = 0 in 
+        let __tmp_2 = (nSCore__List__filter<T=[NSCore__Int, NSCore__Int]>[/Users/joseabelcastellanosjoo/BosqueLanguage/ref_impl/src/test/apps/tictactoe/main.bsq%44%0] __tmp_1 this) in 
+            let __ir_ret__ = __tmp_2 in 
+                let _return_ = __ir_ret__ in 
+                    _return_
+
+val nSMain__id : (x:bosqueTerm{subtypeOf BIntType (getType x)}) -> Tot (x:bosqueTerm{subtypeOf BIntType (getType x)})
+let nSMain__id x = 
+    let __ir_ret__ = x in 
+        let _return_ = __ir_ret__ in 
+            _return_
+
+val nSMain__id : (x:bosqueTerm{subtypeOf BIntType (getType x)}) -> Tot (x:bosqueTerm{subtypeOf BIntType (getType x)})
+let nSMain__id x = 
+    let __ir_ret__ = x in 
+        let _return_ = __ir_ret__ in 
+            _return_
+
+val nSMain__Board__getCellContents : (x:bosqueTerm{subtypeOf BNoneType (getType x)}) -> (x:bosqueTerm{subtypeOf BIntType (getType x)}) -> (x:bosqueTerm{subtypeOf BIntType (getType x)}) -> Tot (x:bosqueTerm{subtypeOf bUnionType_BNoneType_bTypeStringType_BNoneType (getType x)})
+let nSMain__Board__getCellContents this x y = 
+    let _MIRAccessFromField = 0 in 
+        let __tmp_6 = (op_Multiply y 3) in 
+            let __tmp_4 = (op_Addition x __tmp_6) in 
+                let __tmp_3 = (nSCore__List__at<T=NSCore__None|NSCore__String<NSMain__PlayerMark>> __tmp_2 __tmp_4) in 
+                    let __ir_ret__ = __tmp_3 in 
+                        let _return_ = __ir_ret__ in 
+                            _return_
+
+val nSMain__Board__isCellOccupied : (x:bosqueTerm{subtypeOf BNoneType (getType x)}) -> (x:bosqueTerm{subtypeOf BIntType (getType x)}) -> (x:bosqueTerm{subtypeOf BIntType (getType x)}) -> Tot (x:bosqueTerm{subtypeOf BBoolType (getType x)})
+let nSMain__Board__isCellOccupied this x y = 
+    let __tmp_1 = (nSMain__Board__getCellContents this x y) in 
+        let _MIRIsTypeOfSome = 0 in 
+            let __ir_ret__ = __tmp_0 in 
+                let _return_ = __ir_ret__ in 
+                    _return_
+
+val nSMain__Game__makeAutoMove : (x:bosqueTerm{subtypeOf BNoneType (getType x)}) -> (x:bosqueTerm{subtypeOf bTypeStringType_BNoneType (getType x)}) -> (x:bosqueTerm{subtypeOf BIntType (getType x)}) -> Tot (x:bosqueTerm{subtypeOf BNoneType (getType x)})
+let nSMain__Game__makeAutoMove this mark rnd = 
+    let _MIRAccessFromField = 0 in 
+        let __tmp_5 = (nSMain__Board__isCellOccupied __tmp_4 1 1) in 
+            let __tmp_1 = (op_Negation __tmp_5) in 
+                if (op_Equality __tmp_1 true) then 
+                    let _MIRAccessFromField = 0 in 
+                        let __tmp_11 = (nSMain__Board__markCellWith __tmp_10 1 1 mark) in 
+                            let nboard_1 = __tmp_11 in 
+                                let nboard_2 = nboard_1 in 
+                                    let __tmp_34 = (nSMain__Board__checkForWinner nboard_2) in 
+                                        let _MIRModifyWithFields = 0 in 
+                                            let __ir_ret__ = __tmp_32 in 
+                                                let _return_ = __ir_ret__ in 
+                                                    _return_
                 else 
-                    let __ir_ret__ = y in 
-                        let __ir_ret___3 = __ir_ret__ in 
-                            let _return_ = __ir_ret___3 in 
+                    let _MIRAccessFromField = 0 in 
+                        let __tmp_18 = (nSMain__Board__getOpenCells __tmp_17) in 
+                            let opts = __tmp_18 in 
+                                let __tmp_19 = (nSCore__List__uniform<T=[NSCore__Int, NSCore__Int]> opts rnd) in 
+                                    let tup = __tmp_19 in 
+                                        let _MIRAccessFromField = 0 in 
+                                            let _MIRAccessFromIndex = 0 in 
+                                                let _MIRAccessFromIndex = 0 in 
+                                                    let __tmp_25 = (nSMain__Board__markCellWith __tmp_24 __tmp_28 __tmp_29 mark) in 
+                                                        let nboard = __tmp_25 in 
+                                                            let nboard_2 = nboard in 
+                                                                let __tmp_34 = (nSMain__Board__checkForWinner nboard_2) in 
+                                                                    let _MIRModifyWithFields = 0 in 
+                                                                        let __ir_ret__ = __tmp_32 in 
+                                                                            let _return_ = __ir_ret__ in 
+                                                                                _return_
+
+val nSMain__Game__makeExplicitMove : (x:bosqueTerm{subtypeOf BNoneType (getType x)}) -> (x:bosqueTerm{subtypeOf BIntType (getType x)}) -> (x:bosqueTerm{subtypeOf BIntType (getType x)}) -> (x:bosqueTerm{subtypeOf bTypeStringType_BNoneType (getType x)}) -> Tot (x:bosqueTerm{subtypeOf BNoneType (getType x)})
+let nSMain__Game__makeExplicitMove this x y mark = 
+    let _MIRAccessFromField = 0 in 
+        let __tmp_3 = (nSMain__Board__markCellWith __tmp_2 x y mark) in 
+            let nboard = __tmp_3 in 
+                let __tmp_11 = (nSMain__Board__checkForWinner nboard) in 
+                    let _MIRModifyWithFields = 0 in 
+                        let __ir_ret__ = __tmp_9 in 
+                            let _return_ = __ir_ret__ in 
                                 _return_
 
-val nSMain__identityTupleOptional : (x:bosqueTerm{subtypeOf bUnionType_bTupleType_false3(SCons BIntType (SCons BBoolType (SCons BIntType SNil)))_bTupleType_true4(SCons BIntType (SCons BBoolType (SCons BIntType (SCons BBoolType SNil)))) (getType x)}) -> Tot (x:bosqueTerm{subtypeOf bUnionType_bTupleType_false3(SCons BIntType (SCons BBoolType (SCons BIntType SNil)))_bTupleType_true4(SCons BIntType (SCons BBoolType (SCons BIntType (SCons BBoolType SNil)))) (getType x)})
-let nSMain__identityTupleOptional x = 
-    let __ir_ret__ = x in 
-        let _return_ = __ir_ret__ in 
-            _return_
-
-val nSMain__identityOpenTuple : (x:bosqueTerm{isTuple true 1 (SCons bTypeStringType_BAnyType SNil)}) -> Tot (x:bosqueTerm{isTuple true 1 (SCons bTypeStringType_BAnyType SNil)})
-let nSMain__identityOpenTuple x = 
-    let __ir_ret__ = x in 
-        let _return_ = __ir_ret__ in 
-            _return_
-
-val nSMain__main : (x:bosqueTerm{subtypeOf BIntType (getType x)})
+val nSMain__main : (x:bosqueTerm{subtypeOf BNoneType (getType x)})
 let nSMain__main  = 
-    let string_test = "string_test" in 
-        let _LoadConstTypeString = 0 in 
-            let player1 = __tmp_1 in 
-                let n = none in 
-                    let __tmp_3 = (Mktuple__2 10 30) in 
-                        let xTuple2 = __tmp_3 in 
-                            let __tmp_19 = (Mktuple__2 1 1) in 
-                                let __tmp_6 = (Mktuple__16 1 1 1 1 1 1 1 1 1 1 1 1 __tmp_19 "hello" false true) in 
-                                    let x2 = __tmp_6 in 
-                                        let y = 20 in 
-                                            let __tmp_26 = (nSMain__identityUnion y) in 
-                                                let y2 = __tmp_26 in 
-                                                    let _MIRAccessFromIndex = 0 in 
-                                                        let __tmp_28 = (nSMain__max __tmp_31 y) in 
-                                                            let z = __tmp_28 in 
-                                                                let __tmp_33 = (nSMain__max z y) in 
-                                                                    let z_max_func_repeated = __tmp_33 in 
-                                                                        let __tmp_37 = (Mktuple__3 1 true 2) in 
-                                                                            let __tmp_36 = (nSMain__identityTupleOptional __tmp_37) in 
-                                                                                let z2 = __tmp_36 in 
-                                                                                    let __tmp_42 = (Mktuple__1 "hello") in 
-                                                                                        let __tmp_41 = (nSMain__identityOpenTuple __tmp_42) in 
-                                                                                            let z3 = __tmp_41 in 
-                                                                                                let __tmp_44 = (Mktuple__2 xTuple2 y) in 
-                                                                                                    let zTuple2 = __tmp_44 in 
-                                                                                                        let __ir_ret__ = z in 
-                                                                                                            let _return_ = __ir_ret__ in 
-                                                                                                                _return_
+    let __tmp_0 = (nSMain__id 1) in 
+        let x = __tmp_0 in 
+            let _LoadFieldDefaultValue = 0 in 
+                let _LoadFieldDefaultValue = 0 in 
+                    let _ConstructorPrimary = 0 in 
+                        let game = __tmp_2 in 
+                            let _MIRAccessConstantValue = 0 in 
+                                let __tmp_5 = (nSMain__Game__makeAutoMove game __tmp_7 0) in 
+                                    let game_1 = __tmp_5 in 
+                                        let _MIRAccessConstantValue = 0 in 
+                                            let __tmp_9 = (nSMain__Game__makeAutoMove game_1 __tmp_11 1) in 
+                                                let game_2 = __tmp_9 in 
+                                                    let _MIRAccessConstantValue = 0 in 
+                                                        let __tmp_13 = (nSMain__Game__makeAutoMove game_2 __tmp_15 2) in 
+                                                            let game_3 = __tmp_13 in 
+                                                                let _MIRAccessConstantValue = 0 in 
+                                                                    let __tmp_17 = (nSMain__Game__makeExplicitMove game_3 2 0 __tmp_21) in 
+                                                                        let game_4 = __tmp_17 in 
+                                                                            let _MIRAccessConstantValue = 0 in 
+                                                                                let __tmp_22 = (nSMain__Game__makeExplicitMove game_4 2 1 __tmp_26) in 
+                                                                                    let game_5 = __tmp_22 in 
+                                                                                        let __ir_ret__ = game_5 in 
+                                                                                            let _return_ = __ir_ret__ in 
+                                                                                                _return_
 
